code/experimental/rsa/Comparison.fst
@@ -1,0 +1,45 @@
+module Comparison 
+
+open FStar.HyperStack
+open FStar.ST
+open FStar.Buffer
+open FStar.Int.Cast
+
+module U32 = FStar.UInt32
+module U64 = FStar.UInt64
+module I32 = FStar.Int32
+
+type bignum = buffer FStar.UInt64.t
+
+val isMore_loop:
+    a:bignum -> b:bignum{length b = length a} -> count:U32.t{U32.v count <= length a} -> ST bool
+    (requires (fun h -> live h a /\ live h b))
+	(ensures (fun h0 _ h1 -> live h0 a /\ live h0 b))
+let rec isMore_loop a b count =
+    push_frame();
+    let res = 
+    if U32.(count >^ 0ul) then
+    let count = U32.(count -^ 1ul) in
+    let t1 = a.(count) in
+    let t2 = b.(count) in
+    (if not (U64.(t1 =^ t2)) then
+        if U64.(t1 >^ t2) then true else false
+    else isMore_loop a b count)
+    else false in
+    pop_frame();
+    res
+
+(* if a > b then true else false *)
+val isMore:
+    aLen:U32.t -> bLen:U32.t ->
+    a:bignum{length a = U32.v aLen} -> b:bignum{length b = U32.v bLen} -> ST bool
+    (requires (fun h -> live h a /\ live h b))
+	(ensures (fun h0 _ h1 -> live h0 a /\ live h0 b))
+let isMore aLen bLen a b =
+    push_frame();
+    let res =
+    if U32.(aLen >^ bLen) then true 
+    else if U32.(aLen <^ bLen) then false
+         else isMore_loop a b aLen in
+    pop_frame();
+    res
