code/experimental/rsa/Convert.fst
@@ -1,0 +1,73 @@
+module Convert
+
+open FStar.HyperStack
+open FStar.ST
+open FStar.Buffer
+open FStar.Int.Cast
+
+module U32 = FStar.UInt32
+module U8 = FStar.UInt8
+module U64 = FStar.UInt64
+
+type uint8_p = buffer FStar.UInt8.t
+type bignum = buffer FStar.UInt64.t
+
+let bn_bytes = 8ul
+
+(* the length of the message in octets *)
+val get_size_nat: lenText:U32.t -> Tot U32.t
+let get_size_nat lenText =
+     U32.((lenText -^ 1ul) /^ bn_bytes +^ 1ul)
+
+val text_to_nat_loop: 
+    input:uint8_p -> len:U32.t -> res:bignum ->
+    num_words:U32.t{U32.v num_words <= length res} -> m:U32.t -> word:U64.t ->
+    i:U32.t{U32.v i <= length input} -> ST unit
+    (requires (fun h -> live h input /\ live h res))
+    (ensures (fun h0 _ h1 -> live h0 input /\ live h0 res /\ live h1 input /\ live h1 res /\ modifies_1 res h0 h1))
+let rec text_to_nat_loop input len res num_words m word i =
+	if U32.(len >^ 0ul) then
+    let len = U32.(len -^ 1ul) in
+    let tmp = input.(i) in
+	let word = U64.((word <<^ 8ul) |^ uint8_to_uint64 tmp) in
+	let i = U32.(i +^ 1ul) in
+	if U32.(m =^ 0ul) then
+	    let num_words = U32.(num_words -^ 1ul) in
+	    res.(num_words) <- word;
+	    let word = 0uL in
+        let m = U32.(bn_bytes -^ 1ul) in
+	    text_to_nat_loop input len res num_words m word i
+	else
+        text_to_nat_loop input len res num_words U32.(m -^ 1ul) word i
+	else ()
+
+val text_to_nat:
+    input:uint8_p -> len:U32.t{U32.v len = length input} -> res:bignum -> ST unit
+	(requires (fun h -> live h input /\ live h res))
+	(ensures (fun h0 _ h1 -> live h0 input /\ live h0 res /\ live h1 res /\ modifies_1 res h0 h1))
+let text_to_nat input len res =
+    let num_words = get_size_nat len in
+    let m = U32.((len -^ 1ul) %^ bn_bytes) in
+    text_to_nat_loop input len res num_words m 0uL 0ul
+
+val nat_to_text_loop:
+    input:bignum -> res:uint8_p -> i:U32.t -> 
+    j:U32.t{U32.v j <= length res} -> ST unit
+	(requires (fun h -> live h input /\ live h res))
+	(ensures (fun h0 _ h1 -> live h0 input /\ live h0 res /\ live h1 res /\ modifies_1 res h0 h1))
+let rec nat_to_text_loop input res i j =
+    if U32.(i >^ 0ul) then
+    let i = U32.(i -^ 1ul) in
+    let ind = U32.(i /^ bn_bytes) in
+    let l = input.(ind) in
+    let tmp = U32.(i %^ bn_bytes) in (* a bug in F* ? *)
+    res.(j) <- U8.(uint64_to_uint8 (U64.(l >>^ U32.(8ul *^ tmp))) &^ 0xffuy);
+    nat_to_text_loop input res i U32.(j +^ 1ul)
+    else () 
+
+val nat_to_text:
+    input:bignum -> len:U32.t -> res:uint8_p{length res = U32.v len} -> ST unit
+	(requires (fun h -> live h input /\ live h res))
+	(ensures (fun h0 _ h1 -> live h0 input /\ live h0 res /\ live h1 res /\ modifies_1 res h0 h1))
+let nat_to_text input len res = 
+    nat_to_text_loop input res len 0ul
