code/experimental/rsa/Division.fst
@@ -1,0 +1,84 @@
+module Division
+
+open FStar.HyperStack
+open FStar.ST
+open FStar.Buffer
+open FStar.Int.Cast
+
+open Shift 
+open Comparison
+open Addition
+
+module U32 = FStar.UInt32
+module U64 = FStar.UInt64
+
+type bignum = buffer FStar.UInt64.t
+
+let bn_bits2 = 64ul
+
+val bits_to_bn: bits:U32.t -> Tot U32.t 
+let bits_to_bn bits =
+    let to_octets = U32.((bits -^ 1ul) /^ 8ul +^ 1ul) in 
+    U32.((to_octets -^ 1ul) /^ 8ul +^ 1ul)
+
+val correct_top: rLen:U32.t -> r:bignum -> ST U32.t
+    (requires (fun h -> live h r))
+	(ensures (fun h0 _ h1 -> live h0 r /\ live h1 r)) 
+let rec correct_top rLen r = 
+    if U32.(rLen >^ 0ul) then
+    let len = U32.(rLen -^ 1ul) in
+    let tmp = r.(len) in
+    (if U64.(tmp =^ 0uL) then
+        correct_top len r
+    else rLen)
+    else rLen
+
+val remainder_loop: 
+    rLen:U32.t -> modLen:U32.t -> resLen:U32.t ->
+    r_i:bignum{length r_i = U32.v rLen} -> mod:bignum{length mod = U32.v modLen} -> 
+    count:U32.t -> res:bignum{length res = U32.v resLen} -> ST unit
+    (requires (fun h -> live h r_i /\ live h mod /\ live h res))
+	(ensures (fun h0 _ h1 -> live h0 r_i /\ live h0 mod /\  live h0 res /\ live h1 res /\ modifies_1 res h0 h1)) 
+let rec remainder_loop rLen modLen resLen r_i mod count res =
+    push_frame();
+    (if U32.(count >^ 0ul) then
+	
+	let isSet = if U64.(mod.(U32.(modLen -^ 1ul)) =^ 1uL) then 1ul else 0ul in
+    let mod1Len = U32.(modLen -^ isSet) in
+    let mod1 = create 0uL mod1Len in
+    rshift1 modLen mod mod1;
+	
+    (if not (isMore modLen rLen mod r_i) then
+		(let tmp = create 0uL rLen in
+        sub rLen modLen r_i mod tmp; (* TODO: fix the top of tmp and rLen *)
+        let tmpLen = correct_top rLen tmp in
+		let r_i = create 0uL tmpLen in
+        blit tmp 0ul r_i 0ul tmpLen;
+		remainder_loop tmpLen mod1Len resLen r_i mod1 U32.(count -^ 1ul) res)
+	else
+		remainder_loop rLen mod1Len resLen r_i mod1 U32.(count -^ 1ul) res)
+    else
+        let len = if U32.(resLen >^ rLen) then rLen else resLen in
+        blit r_i 0ul res 0ul len);
+    pop_frame()
+
+(* TODO: modBits >= aBits *)
+(* res = a % mod *)
+val remainder: 
+    aBits:U32.t -> modBits:U32.t{U32.(modBits <^ aBits)} -> resLen:U32.t -> 
+    a:bignum{length a = U32.v (bits_to_bn aBits)} -> 
+    mod:bignum{length mod = U32.v (bits_to_bn modBits)} -> 
+    res:bignum{length res = U32.v resLen} -> ST unit
+	(requires (fun h -> live h a /\ live h mod /\ live h res))
+	(ensures (fun h0 _ h1 -> live h0 a /\ live h0 mod /\  live h0 res /\ live h1 res /\ modifies_1 res h0 h1))
+let remainder aBits modBits resLen a mod res =
+    push_frame();
+    let aLen = bits_to_bn aBits in
+    let modLen = bits_to_bn modBits in
+    let k = U32.(aBits -^ modBits) in
+    let modk = U32.((k -^ 1ul) /^ bn_bits2 +^ 1ul) in
+    let mod1Len = U32.(modLen +^ modk) in
+    let mod1 = create 0uL mod1Len in
+    lshift modLen mod k mod1;
+    remainder_loop aLen mod1Len resLen a mod1 k res;
+    pop_frame()
