code/experimental/rsa/Exponentiation.fst
@@ -1,0 +1,69 @@
+module Exponentiation
+
+open FStar.HyperStack
+open FStar.ST
+open FStar.Buffer
+open FStar.Int.Cast
+open FStar.All
+
+open Multiplication
+open Division
+
+module U32 = FStar.UInt32
+module U64 = FStar.UInt64
+
+type bignum = buffer FStar.UInt64.t
+
+let bn_bits2 = 64ul 
+
+(* check if input[ind] is equal to 1 *)
+val bn_bit_is_set:
+    input:bignum -> ind:U32.t{U32.(v (ind /^ bn_bits2)) < length input} -> ST bool
+    (requires (fun h -> live h input))
+    (ensures  (fun h0 r h1 -> live h0 input /\ live h1 input))
+let bn_bit_is_set input ind =
+    push_frame();
+    let i = U32.(ind /^ bn_bits2) in
+    let j = U32.(ind %^ bn_bits2) in
+    let tmp = input.(i) in
+    let res = U64.(((tmp >>^ j) &^ 1uL) =^ 1uL) in
+    pop_frame();
+    res
+
+val mod_exp_loop:
+    modBits:U32.t -> aLen:U32.t -> resLen:U32.t -> 
+    n:bignum -> a:bignum{U32.v aLen = length a} -> b:bignum -> 
+    res:bignum{U32.v resLen = length res} -> count:U32.t{U32.v count < length b} -> ST unit
+    (requires (fun h -> live h n /\ live h a /\ live h b /\ live h res))
+    (ensures  (fun h0 r h1 -> live h1 n /\ live h1 a /\ live h1 b /\ live h1 res /\ modifies_1 res h0 h1))
+let rec mod_exp_loop modBits aLen resLen n a b res count =
+    push_frame();
+    (if U32.(count >^ 0ul) then
+    let count = U32.(count -^ 1ul) in
+    let tmpLen = U32.(2ul *^ resLen) in
+    let tmp = create 0uL tmpLen in
+    let tmpBits = U32.(tmpLen *^ 64ul) in
+    sqr resLen res tmp; remainder tmpBits modBits resLen tmp n res;
+    (if (bn_bit_is_set b count) then
+    let tmpLen = U32.(resLen +^ aLen) in
+    let tmp = create 0uL tmpLen in
+    let tmpBits = U32.(tmpLen *^ 64ul) in
+    mult resLen aLen res a tmp; remainder tmpBits modBits resLen tmp n res);
+    mod_exp_loop modBits aLen resLen n a b res count);
+    pop_frame()
+
+(* res = a ^^ b mod n *)
+val mod_exp:
+    modBits:U32.t -> aLen:U32.t -> bBits:U32.t -> resLen:U32.t -> 
+    n:bignum -> a:bignum{U32.v aLen = length a} -> b:bignum -> 
+    res:bignum{U32.v resLen = length res} -> ST unit
+    (requires (fun h -> live h n /\ live h a /\ live h b /\ live h res))
+    (ensures  (fun h0 r h1 -> live h1 n /\ live h1 a /\ live h1 b /\ live h1 res /\ modifies_1 res h0 h1))
+let mod_exp modBits aLen bBits resLen n a b res =
+    push_frame();
+    let ind = U32.(bBits -^ 1ul) in
+    if (bn_bit_is_set b ind) then
+    blit a 0ul res 0ul aLen
+    else res.(0ul) <- 1uL;
+    mod_exp_loop modBits aLen resLen n a b res ind;
+    pop_frame()
