code/experimental/rsa/Multiplication.fst
@@ -1,0 +1,85 @@
+module Multiplication
+
+open FStar.HyperStack
+open FStar.ST
+open FStar.Buffer
+open FStar.Int.Cast
+
+module U32 = FStar.UInt32
+module U64 = FStar.UInt64
+
+type bignum = buffer FStar.UInt64.t
+
+val mult64: x:U64.t -> y:U64.t -> Tot (U64.t * U64.t) 
+let mult64 x y =
+    let a = U64.(x >>^ 32ul) in
+    let b = U64.(x &^ 0xffffffffuL) in
+    let c = U64.(y >>^ 32ul) in
+    let d = U64.(y &^ 0xffffffffuL) in
+
+    let ac = U64.(a *^ c) in
+    let bc = U64.(b *^ c) in
+    let ad = U64.(a *^ d) in
+    let bd = U64.(b *^ d) in
+
+    let mid = U64.((bd >>^ 32ul) +^ (bc &^ 0xffffffffuL) +^ (ad &^ 0xffffffffuL)) in
+
+    let upper64 = U64.(ac +^ (bc >>^ 32ul) +^ (ad >>^ 32ul) +^ (mid >>^ 32ul)) in
+    let lower64 = U64.((mid <<^ 32ul) |^ (bd &^ 0xffffffffuL)) in
+    (upper64, lower64)
+
+val add64: x:U64.t -> y:U64.t -> Tot (U64.t * U64.t)
+let add64 x y =
+    let res = U64.(x +^ y) in
+    let carry = if U64.(res <^ x) then 1uL else 0uL in
+    (carry, res)
+
+val mult_inner_loop: 
+    aLen:U32.t -> a:bignum{U32.v aLen = length a} -> b:bignum -> 
+    i:U32.t{U32.v i < length b} -> j:U32.t{U32.v j <= length a} ->
+    carry:U64.t -> res:bignum -> ST unit
+    (requires (fun h -> live h a /\ live h b /\ live h res))
+    (ensures  (fun h0 r h1 -> live h1 a /\ live h1 b /\ live h1 res /\ modifies_1 res h0 h1))
+let rec mult_inner_loop aLen a b i j carry res =
+    push_frame();
+    (if U32.(j <^ aLen) then
+    (let (carry1, s1) = mult64 a.(j) b.(i) in
+    let (carry2, s2) = add64 res.(U32.(i +^ j)) s1 in
+    let (carry3, s3) = add64 s2 carry in
+    let carry = U64.(carry1 +^ carry2 +^ carry3) in
+    res.(U32.(i +^ j)) <- s3;
+    mult_inner_loop aLen a b i U32.(j +^ 1ul) carry res)
+    else res.(U32.(i +^ aLen)) <- carry);
+    pop_frame()
+
+val mult_outer_loop:
+    aLen:U32.t -> bLen:U32.t -> 
+    a:bignum{U32.v aLen = length a} -> b:bignum{U32.v bLen = length b} ->
+    i:U32.t{U32.(i <=^ bLen)} -> res:bignum{U32.(v (aLen +^ bLen)) = length res} -> ST unit
+    (requires (fun h -> live h a /\ live h b /\ live h res))
+    (ensures  (fun h0 r h1 -> live h1 a /\ live h1 b /\ live h1 res /\ modifies_1 res h0 h1))
+let rec mult_outer_loop aLen bLen a b i res =
+    push_frame();
+    (if U32.(i <^ bLen) then
+    (mult_inner_loop aLen a b i 0ul 0uL res; 
+    mult_outer_loop aLen bLen a b U32.(i +^ 1ul) res));
+    pop_frame()
+
+(* res = a * b *)
+val mult: 
+    aLen:U32.t -> bLen:U32.t -> 
+    a:bignum{U32.v aLen = length a} -> b:bignum{U32.v bLen = length b} ->
+    res:bignum{U32.(v (aLen +^ bLen)) = length res} -> ST unit
+    (requires (fun h -> live h a /\ live h b /\ live h res))
+    (ensures  (fun h0 r h1 -> live h1 a /\ live h1 b /\ live h1 res /\ modifies_1 res h0 h1))
+let mult aLen bLen a b res =
+    mult_outer_loop aLen bLen a b 0ul res
+
+(* TODO: res = a * a *) 
+val sqr: 
+    aLen:U32.t -> a:bignum{U32.v aLen = length a} -> 
+    res:bignum{length res = U32.(v (2ul *^ aLen))} -> ST unit
+    (requires (fun h -> live h a /\ live h res))
+    (ensures  (fun h0 r h1 -> live h1 a /\ live h1 res /\ modifies_1 res h0 h1))
+let sqr aLen a res = 
+    mult aLen aLen a a res
