code/experimental/rsa/Shift.fst
@@ -1,0 +1,81 @@
+module Shift
+
+open FStar.HyperStack
+open FStar.ST
+open FStar.Buffer
+open FStar.Int.Cast
+
+module U32 = FStar.UInt32
+module U64 = FStar.UInt64
+
+type bignum = buffer FStar.UInt64.t
+
+let bn_bits2 = 64ul
+let bn_tbit = 0x8000000000000000uL
+let bn_mask2 = 0xffffffffffffffffuL
+
+val lshift_loop: 
+    a:bignum -> count:U32.t{U32.v count <= length a} -> nw:U32.t ->
+    lb:U32.t -> res:bignum{U32.(v (count +^ nw)) < length res} -> ST unit
+	(requires (fun h -> live h a /\ live h res))
+	(ensures (fun h0 _ h1 -> live h0 a /\ live h0 res /\ live h1 res /\ modifies_1 res h0 h1))
+let rec lshift_loop a count nw lb res =
+    push_frame();
+    (if U32.(count >^ 0ul) then
+    let count = U32.(count -^ 1ul) in
+    let l = a.(count) in
+    let ind = U32.(nw +^ count +^ 1ul) in
+    let rb = U32.(bn_bits2 -^ lb) in
+    let tmp = res.(ind) in
+    res.(ind) <- U64.(tmp |^ ((l >>^ rb) &^ bn_mask2));
+    res.(U32.(ind -^ 1ul)) <- U64.((l <<^ lb) &^ bn_mask2);
+    lshift_loop a count nw lb res);
+    pop_frame()
+    
+(* res = a << n *)
+val lshift:
+    aLen:U32.t -> a:bignum{length a = U32.v aLen} -> nCount:U32.t ->
+    res:bignum{length res = U32.(v (aLen +^ (nCount /^ bn_bits2) +^ 1ul))} -> ST unit
+	(requires (fun h -> live h a /\ live h res))
+	(ensures (fun h0 _ h1 -> live h0 a /\ live h0 res /\ live h1 res /\ modifies_1 res h0 h1))
+let lshift aLen a nCount res = 
+    push_frame();
+    let nw = U32.((nCount -^ 1ul) /^ bn_bits2 +^ 1ul) in
+    let resLen = U32.(aLen +^ nw) in
+    let lb = U32.(nCount %^ bn_bits2) in
+    (if U32.(lb =^ 0ul) 
+    then blit a 0ul res nw aLen
+    else lshift_loop a aLen nw lb res);
+    pop_frame()
+
+val rshift1_loop: 
+    a:bignum -> carry:U64.t -> ind:U32.t{U32.v ind <= length a} -> 
+    res:bignum{U32.v ind <= length res} -> ST unit
+    (requires (fun h -> live h a /\ live h res))
+	(ensures (fun h0 _ h1 -> live h0 a /\ live h0 res /\ live h1 res /\ modifies_1 res h0 h1))
+let rec rshift1_loop a carry ind res =
+    push_frame();
+    (if U32.(ind >^ 0ul) then
+    let ind = U32.(ind -^ 1ul) in
+    let tmp = a.(ind) in
+    res.(ind) <- U64.(((tmp >>^ 1ul) &^ bn_mask2) |^ carry);
+    let carry = if U64.((tmp &^ 1uL) =^ 1uL) then bn_tbit else 0uL in
+    rshift1_loop a carry ind res);
+    pop_frame()
+
+(* res = a >> 1 *)
+val rshift1:
+    aLen:U32.t -> a:bignum{length a = U32.v aLen} -> 
+    res:bignum{length res = U32.v aLen /\ length res = U32.(v (aLen -^ 1ul))} -> ST unit
+	(requires (fun h -> live h a /\ live h res))
+	(ensures (fun h0 _ h1 -> live h0 a /\ live h0 res /\ live h1 res /\ modifies_1 res h0 h1))
+let rshift1 aLen a res =
+    (* if a = 0 then res = 0 *)
+    push_frame();
+    let i = U32.(aLen -^ 1ul) in 
+    let tmp = a.(i) in
+    let carry = if U64.((tmp &^ 1uL) =^ 1uL) then bn_tbit else 0uL in
+    let tmp = U64.(tmp >>^ 1ul) in
+    (if U64.(tmp >^ 0uL) then res.(i) <- tmp);
+    rshift1_loop a carry i res;
+    pop_frame()
